cfrontend/Csharpminor.v
@@ -392,11 +392,7 @@ Inductive step: state -> trace -> state -> Prop :=
       Genv.find_funct ge vf = Some fd ->
       funsig fd = sig ->
       step (State f (Scall optid sig a bl) k e le m)
-<<<<<<< HEAD
-        E0 (Callstate vf vargs (Kcall optid f e le k) m)
-=======
-        E0 (Callstate fd vargs (Kcall optid f e le k) m id)
->>>>>>> a091c4c
+        E0 (Callstate vf vargs (Kcall optid f e le k) m id)
 
   | step_builtin: forall f optid ef bl k e le m vargs t vres m',
       eval_exprlist e le m bl vargs ->
@@ -458,34 +454,21 @@ Inductive step: state -> trace -> state -> Prop :=
       step (State f (Sgoto lbl) k e le m)
         E0 (State f s' k' e le m)
 
-<<<<<<< HEAD
-  | step_internal_function: forall vf f vargs k m m1 e le,
+  | step_internal_function: forall vf f vargs k m m0 m1 e le id path,
       forall FIND: Genv.find_funct ge vf = Some (Internal f),
-=======
-  | step_internal_function: forall f vargs k m m0 m1 e le id path,
->>>>>>> a091c4c
       list_norepet (map fst f.(fn_vars)) ->
       list_norepet f.(fn_params) ->
       list_disjoint f.(fn_params) f.(fn_temps) ->
       Mem.alloc_frame m id = (m0,path) ->
       alloc_variables empty_env m0 (fn_vars f) e m1 ->
       bind_parameters f.(fn_params) vargs (create_undef_temps f.(fn_temps)) = Some le ->
-<<<<<<< HEAD
-      step (Callstate vf vargs k m)
+      step (Callstate vf vargs k m id)
         E0 (State f f.(fn_body) k e le m1)
 
-  | step_external_function: forall vf ef vargs k m t vres m',
+  | step_external_function: forall vf ef vargs k m t vres m' id,
       forall FIND: Genv.find_funct ge vf = Some (External ef),
       external_call ef ge vargs m t vres m' ->
-      step (Callstate vf vargs k m)
-=======
-      step (Callstate (Internal f) vargs k m id)
-        E0 (State f f.(fn_body) k e le m1)
-
-  | step_external_function: forall ef vargs k m t vres m' id,
-      external_call ef ge vargs m t vres m' ->
-      step (Callstate (External ef) vargs k m id)
->>>>>>> a091c4c
+      step (Callstate vf vargs k m id)
          t (Returnstate vres k m')
 
   | step_return: forall v optid f e le k m,
@@ -499,43 +482,28 @@ End RELSEM.
   corresponding to the invocation of the ``main'' function of the program
   without arguments and with an empty continuation. *)
 
-<<<<<<< HEAD
 Inductive initial_state (ge: genv): c_query -> state -> Prop :=
-  | initial_state_intro: forall vf f vargs m,
+  | initial_state_intro: forall vf f vargs m id,
       Genv.find_funct ge vf = Some (Internal f) ->
       initial_state ge
         (cq vf (fn_sig f) vargs m)
-        (Callstate vf vargs Kstop m).
+        (Callstate vf vargs Kstop m id).
 
 Inductive at_external (ge: genv): state -> c_query -> Prop :=
-  | at_external_intro vf name sg vargs k m:
+  | at_external_intro vf name sg vargs k m id:
       Genv.find_funct ge vf = Some (External (EF_external name sg)) ->
       at_external ge
-        (Callstate vf vargs k m)
+        (Callstate vf vargs k m id)
         (cq vf sg vargs m).
 
 Inductive after_external: state -> c_reply -> state -> Prop :=
-  | after_external_intro vf vargs k m vres m':
+  | after_external_intro vf vargs k m vres m' id:
       after_external
-        (Callstate vf vargs k m)
+        (Callstate vf vargs k m id)
         (cr vres m')
         (Returnstate vres k m').
 
 Inductive final_state: state -> c_reply -> Prop :=
-=======
-Inductive initial_state (p: program): state -> Prop :=
-  | initial_state_intro: forall b f m0,
-      let ge := Genv.globalenv p in
-      Genv.init_mem p = Some m0 ->
-      Genv.find_symbol ge p.(prog_main) = Some b ->
-      Genv.find_funct_ptr ge b = Some f ->
-      funsig f = signature_main ->
-      initial_state p (Callstate f nil Kstop m0 p.(prog_main)).
-
-(** A final state is a [Returnstate] with an empty continuation. *)
-
-Inductive final_state: state -> int -> Prop :=
->>>>>>> a091c4c
   | final_state_intro: forall r m,
       final_state
         (Returnstate r Kstop m)
