cfrontend/Cshmgenproof.v
@@ -1485,25 +1485,16 @@ Inductive match_states: Clight.state -> Csharpminor.state -> Prop :=
       match_states (Clight.State f s k e le m)
                    (State tf ts' tk' te le m)
   | match_callstate:
-<<<<<<< HEAD
-      forall vf fd args k m tfd tk targs tres cconv cu ce
+      forall vf fd args k m tfd tk targs tres cconv cu ce id
           (FS: Genv.find_funct ge vf = Some fd)
           (FT: Genv.find_funct tge vf = Some tfd)
-=======
-      forall fd args k m tfd tk targs tres cconv cu ce id
->>>>>>> a091c4c
           (LINK: linkorder cu prog)
           (TR: match_fundef cu fd tfd)
           (MK: match_cont ce tres 0%nat 0%nat k tk)
           (ISCC: Clight.is_call_cont k)
           (TY: type_of_fundef fd = Tfunction targs tres cconv),
-<<<<<<< HEAD
-      match_states (Clight.Callstate vf args k m)
-                   (Callstate vf args tk m)
-=======
-      match_states (Clight.Callstate fd args k m id)
-                   (Callstate tfd args tk m id)
->>>>>>> a091c4c
+      match_states (Clight.Callstate vf args k m id)
+                   (Callstate vf args tk m id)
   | match_returnstate:
       forall res tres k m tk ce
           (MK: match_cont ce tres 0%nat 0%nat k tk)
@@ -1887,12 +1878,8 @@ Proof.
   econstructor; eauto. constructor.
 
 - (* internal function *)
-<<<<<<< HEAD
   rewrite FS in FIND. inv FIND.
-  inv H. inv TR. monadInv H5.
-=======
   inv H. inv TR. monadInv H6.
->>>>>>> a091c4c
   exploit match_cont_is_call_cont; eauto. intros [A B].
   exploit match_env_alloc_variables; eauto.
   apply match_env_empty.
@@ -1900,19 +1887,12 @@ Proof.
   econstructor; split.
   apply plus_one. eapply step_internal_function; eauto.
   simpl. erewrite transl_vars_names by eauto. assumption.
-<<<<<<< HEAD
-=======
-  simpl. assumption.
-  simpl. assumption.
-  eauto. eauto.
-  simpl; eauto.
->>>>>>> a091c4c
   simpl. rewrite create_undef_temps_match. eapply bind_parameter_temps_match; eauto.
   simpl. econstructor; eauto.
   unfold transl_function. rewrite EQ; simpl. rewrite EQ1; simpl. auto.
   constructor.
   replace (fn_return f) with tres. eassumption.
-  simpl in TY. unfold type_of_function in TY. congruence. 
+  simpl in TY. unfold type_of_function in TY. congruence.
 
 - (* external function *)
   rewrite FS in FIND. inv FIND.
@@ -1921,7 +1901,7 @@ Proof.
   econstructor; split.
   apply plus_one. econstructor; eauto.
   eapply match_returnstate with (ce := ce); eauto.
-  apply has_rettype_wt_val. 
+  apply has_rettype_wt_val.
   replace (rettype_of_type tres0) with (sig_res (ef_sig ef)).
   eapply external_call_well_typed_gen; eauto.
   rewrite H5. simpl. simpl in TY. congruence.
@@ -1945,22 +1925,10 @@ Lemma transl_initial_states:
   exists R, initial_state tge q R /\ match_states S R.
 Proof.
   intros. inv H.
-<<<<<<< HEAD
   exploit functions_translated; eauto. intros (cu & tf & A & B & C).
   eexists. split.
   - erewrite <- transl_fundef_sig2 by eauto. inv B. econstructor; eauto.
   - eapply match_callstate with (ce := genv_cenv ge); eauto; constructor.
-=======
-  exploit function_ptr_translated; eauto. intros (cu & tf & A & B & C).
-  assert (D: Genv.find_symbol tge (AST.prog_main tprog) = Some b).
-  { destruct TRANSL as (P & Q & R). rewrite Q. rewrite symbols_preserved. auto. }
-  assert (E: funsig tf = signature_of_type Tnil type_int32s cc_default).
-  { eapply transl_fundef_sig2; eauto. }
-  econstructor; split.
-  econstructor; eauto. apply (Genv.init_mem_match TRANSL). eauto.
-  destruct TRANSL as (P & Q & R). rewrite Q.
-  econstructor; eauto. instantiate (1 := prog_comp_env cu). constructor; auto. exact I.
->>>>>>> a091c4c
 Qed.
 
 Lemma transl_external:
