cfrontend/SimplExprproof.v
@@ -1126,20 +1126,11 @@ Inductive match_states: Csem.state -> state -> Prop :=
       (MK: match_cont cu.(prog_comp_env) k tk),
       match_states (Csem.State f s k e m)
                    (State tf ts tk e le m)
-<<<<<<< HEAD
-  | match_callstates: forall vf args k m tk cu
-=======
-  | match_callstates: forall fd args k m tfd tk cu id
->>>>>>> a091c4c
+  | match_callstates: forall vf args k m tk cu id
       (LINK: linkorder cu prog)
       (MK: forall ce, match_cont ce k tk),
-<<<<<<< HEAD
-      match_states (Csem.Callstate vf args k m)
-                   (Callstate vf args tk m)
-=======
-      match_states (Csem.Callstate fd args k m id)
-                   (Callstate tfd args tk m id)
->>>>>>> a091c4c
+      match_states (Csem.Callstate vf args k m id)
+                   (Callstate vf args tk m id)
   | match_returnstates: forall res k m tk
       (MK: forall ce, match_cont ce k tk),
       match_states (Csem.Returnstate res k m)
@@ -2353,22 +2344,13 @@ Proof.
   econstructor; eauto.
 
 - (* internal function *)
-<<<<<<< HEAD
   edestruct functions_translated as (cu' & tfd & FIND' & TF & CU); eauto.
-  inv TF. inversion H3; subst.
+  inv TF. inversion H4; subst.
   econstructor; split.
   left; apply plus_one. eapply step_internal_function; eauto. econstructor.
-  rewrite H6; rewrite H7; auto.
-  rewrite H6; rewrite H7. eapply alloc_variables_preserved; eauto.
-  rewrite H6. eapply bind_parameters_preserved; eauto.
-=======
-  inv TR. inversion H4; subst.
-  econstructor; split.
-  left; apply plus_one. eapply step_internal_function. econstructor.
   rewrite H7; rewrite H8; eauto. eauto.
   rewrite H7; rewrite H8. eapply alloc_variables_preserved; eauto.
   rewrite H7. eapply bind_parameters_preserved; eauto.
->>>>>>> a091c4c
   eauto.
   econstructor; eauto.
 
@@ -2407,12 +2389,11 @@ Lemma transl_initial_states:
   exists S', Clight.initial_state tge q S' /\ match_states S S'.
 Proof.
   intros. inv H.
-<<<<<<< HEAD
   exploit functions_translated; eauto. intros (cu & tf & FIND & TR & L).
   econstructor; split.
   - inversion TR; subst.
     econstructor; eauto.
-    rewrite <- H1. apply (type_of_fundef_preserved cu (Internal f) (Internal tf0)). auto.
+    rewrite <- H2. apply (type_of_fundef_preserved cu (Internal f) (Internal tf0)). auto.
   - econstructor; eauto. constructor.
 Qed.
 
@@ -2426,19 +2407,6 @@ Proof.
   edestruct functions_translated as (cu' & tfd & Htfd & TR & L); eauto. inv TR.
   split. econstructor; eauto. intros r S' HS'. inv HS'.
   eexists. split; econstructor; eauto.
-=======
-  exploit function_ptr_translated; eauto. intros (cu & tf & FIND & TR & L).
-  destruct TRANSL. destruct H as (A & B & C).
-  econstructor; split.
-  econstructor.
-  eapply (Genv.init_mem_match (proj1 TRANSL)); eauto.
-  setoid_rewrite B.
-  rewrite symbols_preserved. eauto.
-  eexact FIND.
-  rewrite <- H3. eapply type_of_fundef_preserved; eauto.
-  setoid_rewrite B.
-  econstructor; eauto. intros; constructor.
->>>>>>> a091c4c
 Qed.
 
 Lemma transl_final_states:
